Logic.v
@@ -1,0 +1,197 @@
+Require Import ACTL.
+Require Import EDEN.
+Require Import Coq.Setoids.Setoid.
+
+
+
+Set Implicit Arguments.
+
+
+
+Notation "s |= f" := (@sat State action Trans f s)(at level 80).
+Notation "|= f" := (forall s, s |= f)(at level 80).
+Notation τ := (action_ tau).
+Notation "< chi > f" := (E (⊤ [τ] U [chi] f))(at level 50, chi at level 5).
+Notation "[ chi ] f" := (¬ <chi> ¬ f)(at level 50, chi at level 5).
+Notation "'EX' f" := (<any> f)(at level 50).
+Notation "'AX' f" := ([any] f)(at level 50).
+Notation "'EF' f" := (f ∨ EF [any] f)(at level 50).
+Notation "'AF' f" := (f ∨ AF [any] f)(at level 50).
+Notation "'EG' f" := (¬ AF ¬ f)(at level 50).
+Notation "'AG' f" := (¬ EF ¬ f)(at level 50).
+
+
+Notation "f 'EU' f'" := (f' ∨ (f ∧ (EX (E (f U f')))))(at level 50).
+Notation "f 'AU' f'" := (f' ∨ (f ∧ (AX (A (f U f')))))(at level 50).
+Notation "f 'EW' f'" := (¬ ((¬ f') AU ((¬ f) ∧ (¬ f'))))(at level 50).
+Notation "f 'AW' f'" := (¬ ((¬ f') EU ((¬ f) ∧ (¬ f'))))(at level 50).
+
+Notation Path := (@path State action Trans).
+Notation Form := (@form action).
+Notation Formr := (@formr action).
+
+Notation Action_ := (@action_ action).
+Notation Act_var := (@act_var Proposal).
+
+
+(* 命題変数 *)
+Notation HasNoBudget adm := (<(Action_ (Act_var (hasNoBudget adm)))> ⊤).
+Notation HasNoComitee adm := (<(Action_ (Act_var (hasNoComitee adm)))> ⊤).
+Notation HasNoTenureWoker adm := (<(Action_ (Act_var (hasNoTenureWoker adm)))> ⊤).
+Notation HasNoMember adm := (<(Action_ (Act_var (hasNoMember adm)))> ⊤).
+Notation IsBudgetRestricted adm := (<(Action_ (Act_var (isBudgetRestricted adm)))> ⊤).
+Notation IsTransferRestricted adm := (<(Action_ (Act_var (isBudgetRestricted adm)))> ⊤).
+Notation IsAssignmentRestrected adm adm' := (<(Action_ (Act_var (isAssignmentRestrected adm adm')))> ⊤).
+Notation IsAdminControlRestricted adm := (<(Action_ (Act_var (isAdminControlRestricted adm)))> ⊤).
+Notation IsAssigned adm ctz := (<(Action_ (Act_var (isAssigned adm ctz)))> ⊤).
+Notation IsProposed adm prp := (<(Action_ (Act_var (isProposed adm prp)))> ⊤).
+Notation IsTenureWorker adm ctz := (<(Action_ (Act_var (isTenureWorker adm ctz)))> ⊤).
+Notation IsWithinExpiration adm ctz := (<(Action_ (Act_var (isWithinExpiration adm ctz)))> ⊤).
+
+
+Notation Propose prp := (Action_ (act_proposal prp)).
+Notation Withdraw adm n := (Propose (withdraw adm n)).
+Notation Deposit adm n := (Propose (deposit adm n)).
+Notation Transfer from to n := (Propose (transfer from to n)).
+Notation AssignMember adm n := (Propose (assignMember adm n)).
+Notation DismissalMember adm n := (Propose (dismissalMember adm n)).
+Notation AssignTenureWorker adm n := (Propose (withdraw adm n)).
+Notation DismissalTenureWorker adm n := (Propose (dismissalTenureWorker adm n)).
+Notation GenAdmin adm n := (Propose (genAdmin adm n)).
+Notation SlashAdmin adm n := (Propose (slashAdmin adm n)).
+
+Notation Deliberate adm := (Action_ (act_deliberate adm)).
+
+
+Definition ROOT := Adm 0.
+Definition PROFESSIONALS := Adm 1.
+Definition FACILITATORS := Adm 2.
+Definition REGISTRATOR := Adm 3.
+Definition POLICE := Adm 4.
+(* Definition JUDICIARY := Adm 5.
+Definition MILITARY := Adm 6.
+Definition MEDIA := Adm 7.
+Definition EDUCATION := Adm 8. *)
+
+
+Definition IsAssignmentRestrectedStrict adm :=
+    IsAssignmentRestrected adm ROOT ∧
+    IsAssignmentRestrected adm PROFESSIONALS ∧
+    IsAssignmentRestrected adm FACILITATORS ∧
+    IsAssignmentRestrected adm POLICE.
+    (* IsAssignmentRestrected adm JUDICIARY ∧
+    IsAssignmentRestrected adm MILITARY ∧   
+    IsAssignmentRestrected adm MEDIA ∧   
+    IsAssignmentRestrected adm EDUCATION. *)
+
+
+
+
+
+Definition ROOT_spec :=
+    IsBudgetRestricted ROOT ∧
+    HasNoTenureWoker ROOT ∧
+    IsAssignmentRestrected ROOT ROOT.
+
+    
+Definition PROFESSIONAL_spec :=
+    HasNoBudget PROFESSIONALS ∧
+    HasNoComitee PROFESSIONALS ∧
+    HasNoMember PROFESSIONALS.
+
+Definition FACILITATORS_spec :=
+    HasNoBudget FACILITATORS ∧
+    HasNoComitee FACILITATORS ∧
+    HasNoMember FACILITATORS.
+
+    
+Definition REGISTRATOR_spec :=
+    IsBudgetRestricted REGISTRATOR ∧
+    IsTransferRestricted REGISTRATOR ∧
+    IsAdminControlRestricted REGISTRATOR ∧
+    IsAssignmentRestrected REGISTRATOR REGISTRATOR ∧
+    IsAssignmentRestrected REGISTRATOR FACILITATORS ∧
+    IsAssignmentRestrected REGISTRATOR REGISTRATOR ∧
+    IsAssignmentRestrected REGISTRATOR POLICE.
+
+Definition POLICE_spec :=
+    IsBudgetRestricted POLICE ∧
+    IsTransferRestricted POLICE ∧
+    IsAdminControlRestricted POLICE ∧
+    IsAssignmentRestrected POLICE ROOT ∧
+    IsAssignmentRestrected POLICE PROFESSIONALS ∧
+    IsAssignmentRestrected POLICE FACILITATORS ∧
+    IsAssignmentRestrected POLICE REGISTRATOR ∧
+    IsAssignmentRestrected POLICE POLICE.
+
+
+Definition SPEC :=
+    ROOT_spec ∧ PROFESSIONAL_spec ∧ REGISTRATOR_spec ∧ POLICE_spec.
+
+Ltac  satisfy := unfold sat; fold (sat (trans := Trans)).
+
+Theorem tau_eq : forall  s s', Trans s tau s' <->  s = s'.
+Proof.
+    intros s s'; split; intro H; symmetry; auto.    
+Qed.
+
+Theorem IsAssignedUnfdold adm c s :
+    s |= IsAssigned adm c  <-> 
+        match Ssubstate s adm with 
+        | None => False 
+        | Some ss' => c \in SSmember ss'
+        end.
+Proof.
+    split; satisfy; intro H.
+    -   induction H as [r [Hr [_ HU]]].
+        induction HU; simpl in *; subst; auto; simpl in *.
+        +   destruct r, p; simpl in *; subst;
+                inversion t; subst; destruct s'; auto.
+        +   apply IHHU; auto.
+    -   remember (Ssubstate s adm) as ss.
+        destruct ss.
+        +   assert (Trans s (Act_var (isAssigned adm c)) s) as Ht.
+            { constructor; simpl; destruct (Ssubstate s adm);
+                inversion Heqss; subst; auto.
+            }    
+            Check path.
+
+            exists (Run s (nilp s (Act_var (isAssigned adm c)) s Ht));
+            repeat split; constructor; unfold sata; auto.
+        +   inversion H.
+Qed.
+
+Theorem IsProposedUnfold adm prp s : 
+            s |= IsProposed adm prp <->
+                match Ssubstate s adm with 
+                | None => False 
+                | Some ss => match SScomitee ss with
+                    | None => False 
+                    | Some cmt => prp =  Dproposal cmt
+                    end
+                end.
+Proof.
+    split; satisfy; intro H.
+    -   induction H as [r [Hr [_ HU]]].
+        induction HU; simpl in *; subst; auto; simpl in *.
+        +   destruct r, p; simpl in *; subst;
+                inversion t; subst; destruct s'; auto.
+        +   apply IHHU; auto.
+    -   remember (Ssubstate s adm) as ss.
+        destruct ss.
+        +   assert (Trans s (Act_var (isProposed adm prp)) s) as Ht.
+            { constructor; simpl; destruct (Ssubstate s adm);
+                inversion Heqss; subst; auto.
+            }            
+            exists (Run s (nilp s (Act_var (isProposed adm prp)) s Ht));
+            repeat split; constructor; unfold sata; auto.
+        +   inversion H.
+Qed.            
+
+            
+Definition dismissible adm c :=
+    (IsProposed ROOT (dismissalMember adm c)) ∧ ¬ [Deliberate ROOT] (IsAssigned adm c).
+
+    
+Definition deliberate_soundness adm c :=
+    |= IsAssigned adm c → AF (dismissible adm c).
